# 제어공학1_HW1

### P2.7

$$
\begin{aligned}
I = \frac{V_1(s)}{R}=-C\frac{dV_2(s)}{dt}
\end{aligned}
$$

##### Laplace Transform

$$
\begin{aligned}
\frac{V_1(s)}{R} = -CsV_2(s)
\end{aligned}
$$

$$
\begin{aligned}
\therefore  \frac{V_2(s)}{V_1(s)} = - \frac{1}{RCs}
\end{aligned}
$$


### P2.12

$$
\begin{aligned}
G(s) = K \frac {1}{s+50}
\end{aligned}
$$

$$
\begin{aligned}
Y(s) = R(s)G(s)
\end{aligned}
$$

##### Laplace Transform

$$
\begin{aligned}
r(t) = 1 ⟶ R(s) = \frac {1}{s}
\end{aligned}
$$

$$
\begin{aligned}
Y(s) = \frac{1}{s} K \frac {1}{s+50} = \frac{k}{s(s+50)} = \frac {A}{s} + \frac{B}{s+50}
\end{aligned}
$$
\
$$
\begin{aligned}
As + Bs = 0s \longrightarrow A = -B
\end{aligned}
$$

$$
\begin{aligned}
50A = K \longrightarrow A = \frac{K}{50}, B = -\frac{K}{50}
\end{aligned}
$$

$$
\begin{aligned}
Y(s) = \frac{K}{50}\frac{1}{s} - \frac{k}{50}\frac{1}{s+50} = \frac{K}{50} (\frac{1}{s} - \frac{1}{s+50})
\end{aligned}
$$

##### Inverse Laplace Transform

$$
\begin{aligned}
y(t) = \frac{K}{50}(1-e^{-50t}) (t ≥ 0)
\end{aligned}
$$

$$
\begin{aligned}
\lim_{t \to 0} y(t) = 1 = \frac{K}{50}(1-e^{-50t})
\end{aligned}
$$

$$
\begin{aligned}
\therefore K = 50
\end{aligned}
$$


### P2.26

$$
\begin{aligned}
Mx''(t) = F(t) - b(x'(t)-y'(t))-k(x(t)-y(t))
\end{aligned}
$$
\
$$
\begin{aligned}
my''(t) = b(x'(t)-y'(t))+k(x(t)-y(t))
\end{aligned}
$$

[초기조건은 0이라 가정]

##### Laplace Transform

$$
\begin{aligned}
Ms^2X(s) = F(s) - bs(X(s)-Y(s))-k(X(s)-Y(s)) - 식①
\end{aligned}
$$

$$
\begin{aligned}
ms^2Y(s) = bs(X(s)-Y(s)) + k(X(s)-Y(s)) - 식②
\end{aligned}
$$
\
$$
\begin{aligned}
식①\ 정리: X(s)(Ms^2+bs+k) - Y(s)(bs+k) = F(s)
\end{aligned}
$$
\
$$
\begin{aligned}
식②\ 정리: Y(s)(ms^2+bs+k) - X(s)(bs-k) = 0
\end{aligned}
$$
\
$$
\begin{aligned}
\therefore Y(s) = \frac{bs+k}{ms^2+bs+k}X(s)
\end{aligned}
$$
\
②를 ①에 대입
\
$$
\begin{aligned}
X(s)(Ms^2+bs+k)-\frac{(bs+k)^2}{ms^2+bs+k}X(s) = F(s)
\end{aligned}
$$
\
$$
\begin{aligned}
X(s)((Ms^2+bs+k)-\frac{(bs+k)^2}{ms^2+bs+k}) = F(s)
\end{aligned}
$$
\
$$
\begin{aligned}
X(s) = F(s)\frac{1}{(Ms^2+bs+k)-\frac{(bs+k)^2}{ms^2+bs+k}} - 식③
\end{aligned}
$$
\
식③을 식②에 대입
$$
\begin{aligned}
\therefore \frac{Y(s)}{F(s)} = \frac{bs+k}{ms^2+bs+k} \frac{1}{(Ms^2+bs+k)-\frac{(bs+k)^2}{ms^2+bs+k}} = \frac{bs+k}{(Ms^2+bs+k)(ms^2+bs+k)-(bs+k)^2}
\end{aligned}
$$


### P2.37


### (a)

$$
\begin{aligned}
m_1x''(t) = -k_1x(t) - k_2(x(t)-y(t))
\end{aligned}
$$
\
$$
\begin{aligned}
m_2y''(t) = -k_2(y(t)-x(t))+u(t)
\end{aligned}
$$

##### Laplace Transform

$$
\begin{aligned}
m_1s^2X(s) = -k_1X(s) -k_2(X(s)-Y(s))
\end{aligned}
$$

$$
\begin{aligned}
m_2Y(s) = -k_2(Y(s)-X(s)) +U(s)
\end{aligned}
$$
\
$$
\begin{aligned}
s^2X(s) + 2X(s) = Y(s) → ①
\end{aligned}
$$
\
$$
\begin{aligned}
s^2Y(s) + Y(s) = X(s) + U(s) → ②
\end{aligned}
$$
\
$$
\begin{aligned}
X(s) = \frac {Y(s)}{s^2+2}
\end{aligned}
$$
\
$$
\begin{aligned}
Y(s)(s^2+1) = X(s) + U(s)
\end{aligned}
$$
\
①을 ②에 대입
$$
\begin{aligned}
(s^2+2)(s^2+1)Y(s) - Y(s) = (s^2+1)U(s)
\end{aligned}
$$


### (b)
$$
\begin{aligned}
\therefore \frac{Y(s)}{U(s)} = \frac{s^2+2}{s^4+3s^2+1}
\end{aligned}
$$
