# 제어공학1_HW3

### P3.1

#### (a)



$$
\begin{aligned}
x_1(t) = y(t)
\end{aligned}
$$
\
$$
\begin{aligned}
x_2(t) = y'(t)
\end{aligned}
$$

#### (b)

$$
\begin{aligned}
M \frac {d^2y(t)}{dt^2} = F(t) - b\frac{dy(t)}{dt} - ky(t)
\end{aligned}
$$
\
$$
\begin{aligned}
x_1'(t) = x_2(t)
\end{aligned}
$$
\
$$
\begin{aligned}
x'_2(t) = \frac{1}{M}[F(t)-bx_2(t)-kx_1(t)]
\end{aligned}
$$

#### (c)

$$\begin{aligned} \therefore X(t) = \end{aligned} \quad \begin{bmatrix} x_1(t) \\x_2(t) \end{bmatrix} \quad \begin{aligned} = \end{aligned} \begin{bmatrix} y(t) \\y'(t) \end{bmatrix}$$

$$\hspace{170pt} \begin{aligned} ⇒ X'(t) = \end{aligned} \quad \begin{bmatrix} x_1'(t) \\ x_2'(t) \end{bmatrix} \quad \begin{aligned} = \end{aligned} \begin{bmatrix} x_2(t) \\ \frac{1}{M}[F(t)-bx_2(t)-kx_1(t)] \end{bmatrix} $$

$$\hspace{170pt} \begin{aligned} ⇒ X'(t) = \end{aligned} \quad \begin{bmatrix} x_1'(t) \\ x_2'(t) \end{bmatrix} \quad \begin{aligned} = \end{aligned} \begin{bmatrix} 0 & 1 \\ -\frac{k}{M} & -\frac{b}{M} \end{bmatrix} \begin{aligned} X(t) + 
 \end{aligned} \begin{bmatrix} 0 \\ \frac{1}{M} \end{bmatrix} \begin{aligned} F(t) \end{aligned} $$

### P3.3

$$\begin{aligned} x_1(t) = i_L(t), x_2(t) = y'(t) \end{aligned}$$

$$\begin{aligned} V_L = L\frac{di_L(t)}{dt} = L\frac{dx_1(t)}{dt} \end{aligned}$$

$$\begin{aligned} i_c(t) = C\frac{dv_c(t)}{dt},V_L(t)=L\frac{di_L(t)}{dt} \end{aligned}$$

$$\begin{aligned} V_1(t) = V_L(t) - V_c(t) + V_2(t) \end{aligned}$$

$$\begin{aligned} V_L(t) = V_1(t) - V_2(t) + V_c(t) \end{aligned}$$

$$\begin{aligned} \therefore \frac{dx_1(t)}{dt} = \frac{1}{L}[V_1(t)-V_2(t)+x_2(t)] \end{aligned}$$

$$\begin{aligned} i_c(t) = -C\frac{dV_c(t)}{dt} = i_L(t) = \frac{V_2(t)-V_c(t)}{R} \end{aligned}$$

$$\begin{aligned} \therefore \frac{dx_2(t)}{dt} = -\frac{1}{C}[x_1(t)-\frac{V_2(t)-x_2(t)}{R}] \end{aligned}$$

$$\hspace{170pt} \begin{aligned} \therefore X(t) = \end{aligned} \quad \begin{bmatrix} x_1(t) \\ x_2(t) \end{bmatrix} \quad \begin{aligned} =   \end{aligned} \begin{bmatrix} i_L(t) \\ V_c(t) \end{bmatrix}$$

$$\hspace{80pt} \begin{aligned} ⇒ X'(t) = \end{aligned} \quad \begin{bmatrix} x_1'(t) \\ x_2'(t) \end{bmatrix} \quad \begin{aligned} = \end{aligned} \begin{bmatrix} 0 & \frac{1}{L} \\ -\frac{1}{C} & -\frac{1}{RC} \end{bmatrix} X(t) + \begin{bmatrix} \frac{1}{L} & -\frac{1}{L} \\ 0 & \frac{1}{RC} \end{bmatrix} V(t)\ =AX(t) + \begin{bmatrix} \frac{1}{L} & -\frac{1}{L} \\ 0 & \frac{1}{RC} \end{bmatrix} V(t)$$


### P3.5


### (a)
\
$$
\begin{aligned}
T(s) = \frac{Y(s)}{R(s)}
\end{aligned}
$$
\
$$
\begin{aligned}
Y(s) = [R(s)-Y(s)][\frac{s+2}{s+8}\frac{1}{s-3}\frac{1}{s}]
\end{aligned}
$$
\
$$
\begin{aligned}
A = \frac{s+2}{s+8}\frac{1}{s-3}\frac{1}{s}
\end{aligned}
$$
\
$$
\begin{aligned}
Y(s)(1+A) = AR(s)
\end{aligned}
$$
\
$$
\begin{aligned}
\therefore \frac{Y(s)}{R(s)} = \frac{A}{1+A} = \frac{\frac{s+2}{s+8}\frac{1}{s-3}\frac{1}{s}}{1+\frac{s+2}{s+8}\frac{1}{s-3}\frac{1}{s}}
\end{aligned}
$$
\
$$
\begin{aligned}
\therefore T(s) = \frac{s+2}{(s+8)(s-3)s+(s+2)}
\end{aligned}
$$

### (b)
\
$$
\begin{aligned}
V_1(s) = \frac{s+2}{s+8}[R(s)-Y(s)]
\end{aligned}
$$
\
$$
\begin{aligned}
\therefore (s+8)V_1(s) = (s+2)[R(s)-Y(s)]
\end{aligned}
$$


#### 제어기 Inverse Laplace

$$
\begin{aligned}
\frac{dV_1(t)}{dt} + 8V_1(t) = \frac{d}{dt}[r(t)-y(t)]+2[r(t)-y(t)]
\end{aligned}
$$
\
$$
\begin{aligned}
V_1'(t) = -8V_1(t) + r'(t) - y'(t) + 2r(t) - 2y(t)
\end{aligned}
$$
\
$$
\begin{aligned}
V_1(t) = x_1(t)
\end{aligned}
$$
\
$$
\begin{aligned}
x_1'(t) = -8x_1(t) + r'(t) - y'(t) + 2[r(t) - y(t)]
\end{aligned}
$$




#### 속도V(s)
\
$$
\begin{aligned}
V(s) = \frac{1}{s-3}V_1(s)
\end{aligned}
$$
\
$$
\begin{aligned}
V(t) = x_2(t)
\end{aligned}
$$


#### Inverse Laplace


$$
\begin{aligned}
x_2'(t) = 3x_2(t) + x_1(t)
\end{aligned}
$$


#### 위치



$$
\begin{aligned}
Y(s) = \frac{1}{s} V(s)
\end{aligned}
$$

#### Inverse Laplace


$$
\begin{aligned}
y(t) = x_3(t)
\end{aligned}
$$
\
$$
\begin{aligned}
x_3'(t) = x_2(t)
\end{aligned}
$$


$$\hspace{110pt} \begin{aligned} \therefore X'(t) = \end{aligned} \quad \begin{bmatrix} -8 & 0 & -2 \\ 1 & 3 & 0 \\ 0 & 1 & 0 \end{bmatrix} \quad \begin{aligned} X(t) + \end{aligned} \begin{bmatrix} 2 \\ 0 \\ 0 \end{bmatrix} r(t) + \begin{bmatrix} -2 \\ 0 \\ 0 \end{bmatrix} y(t)$$


$$\hspace{200pt} \therefore y(t) = \begin{bmatrix} 0 & 0 & 1 \end{bmatrix} X(t)$$


### P3.12

### (a)

$$\begin{aligned} \frac{Y(s)}{R(s)} = T(s) = \frac{8(s+5)}{s^3+12s^2+44s+48} \end{aligned}$$


$$\begin{aligned} x_1(t) = y(t), x_2(t) = y'(t), x_3(t) = y''(t) \end{aligned}$$

$$\begin{aligned} x_1'(t) = x_2(t), x_2'(t) = x_3(t) \end{aligned}$$


#### Inverse Laplace


$$\begin{aligned} y'''(t) + 12y''(t) + 44y'(t) + 48y(t) = 8r'(t) + 40r(t) \end{aligned}$$


$$\begin{aligned} x_3'(t) = -48x_1(t) - 44x_2(t) - 12x_3(t) +8r'(t) +40r(t) \end{aligned}$$


$$\hspace{100pt} \begin{aligned} \therefore X'(t) = \end{aligned} \quad \begin{bmatrix} 0 & 1 & 0 \\ 0 & 0 & 1 \\ -48 & -44 & -12 \end{bmatrix} \quad \begin{aligned} X(t) + \end{aligned} \begin{bmatrix} 0 \\ 0 \\ 40 \end{bmatrix} r(t) + \begin{bmatrix} 0 \\ 0 \\ 8 \end{bmatrix} r'(t)$$


### (b)

$$\hspace{200pt} A= \quad \begin{bmatrix} 0 & 1 & 0 \\ 0 & 0 & 1 \\ -48 & -44 & -12 \end{bmatrix}$$


$$\hspace{100pt} sI-A = \begin{bmatrix} s & 0 & 0 \\ 0 & s & 0 \\ 0 & 0 & s \end{bmatrix} - \begin{bmatrix} 0 & 1 & 0 \\ 0 & 0 & 1 \\ -48 & -44 & -12 \end{bmatrix} = \begin{bmatrix} s & -1 & 0 \\ 0 & s & -1 \\ 48 & 44 & s+12 \end{bmatrix}$$


$$\hspace{110pt} (sI-A)^{-1} = \frac{1}{(s+2)(s+4)(s+6)} \begin{bmatrix} S^2+12s+44 & s+12 & 1 \\ -48 & s^2+12s & s \\ -48s & -(44s+48) & s^2 \end{bmatrix}$$


#### Inverse Laplace
$$\hspace{50pt} Φ(t) = \begin{bmatrix} 3e^{-2t}-3e^{-4t}+e^{-6t} & \frac{5}{4}e^{-2t}-2e^{-4t}+\frac{3}{4}e^{-6t} & \frac{1}{8}e^{-2t} - \frac{1}{4}e^{-4t} + \frac{1}{8}e^{-6t}\\-6e^{-2t}+12e^{-4t}-6e^{-6t} & -\frac{5}{2}e^{-2t}+8e^{-4t}-\frac{9}{2}e^{-6t} & -\frac{1}{4}e^{-2t} + e^{-4t} -\frac{3}{4}e^{-6t} \\ 12e^{-2t} -48e^{-4t}+36e^{-6t} & 5e^{-2t}-32e^{-4t}+27e^{-6t} & \frac{1}{2}e^{-2t}-\frac{1}{4}e^{-4t}+\frac{9}{2}e^{-6t} \end{bmatrix}$$


### P3.17

$$\hspace{170pt} \begin{aligned} X'(t) = \end{aligned} \quad \begin{bmatrix} 1 & 1 & -1 \\ 4 & 3 & 0 \\ -2 & 1 & 10 \end{bmatrix} \quad \begin{aligned} X(t) + \end{aligned} \begin{bmatrix} 0 \\ 0 \\ 4 \end{bmatrix} u(t)$$


$$\hspace{210pt} \begin{aligned} Y(t) = \end{aligned} \quad \begin{bmatrix} 1 & 0 & 0 \end{bmatrix} X(t)$$


### Laplace Transform


$$\hspace{185pt} sX(s) = \begin{bmatrix} 1 & 1 & -1 \\ 4 & 3 & 0 \\ -2 & 1 & 10 \end{bmatrix} X(s) + \begin{bmatrix} 0 \\ 0 \\ 4 \end{bmatrix} U(s)$$


$$\hspace{220pt} \begin{aligned} Y(s) = \end{aligned} \quad \begin{bmatrix} 1 & 0 & 0 \end{bmatrix} X(s)$$


$$\hspace{215pt} \begin{aligned} (sI-A)X(s) = \end{aligned} \begin{bmatrix} 0\\0\\4 \end{bmatrix} U(s)$$


$$\hspace{210pt} X(s) = (sI-A)^{-1} \begin{bmatrix} 0\\0\\4 \end{bmatrix} U(s)$$


$$\hspace{80pt} \frac{Y(s)}{U(s)} = \begin{bmatrix} 1 & 0 & 0 \end{bmatrix} (sI-A)^{-1} \begin{bmatrix} 0\\0\\4 \end{bmatrix} \quad = \begin{bmatrix} 1 & 0 & 0 \end{bmatrix} \quad \begin{bmatrix} s-1 & -1 & 1 \\ -4 & s-3 & 0 \\ 2 & -1 & s-10 \end{bmatrix} \begin{bmatrix} 0\\0\\4 \end{bmatrix} =\frac{-4s+12}{s^3-14s^2+37s+20}$$
